got match vals through untyped combined. This is insane but getting faster

src/UntypedCompCombined.v
@@ -18,23 +18,245 @@ Require
     UntypedComp8
 .
 
+
+
+
+
+Definition compile_13 (cu : Untyped1.env * list metadata) : res (Untyped3.env * list metadata) :=
+  OK cu
+     @@ UntypedComp2.compile_cu
+     @@ UntypedComp3.compile_cu.
+
+Section FSIM13.
+
+
+  Variable a : Untyped1.env * list metadata.
+  Variable b : Untyped3.env * list metadata.
+  Hypothesis TRANSF : compile_13 a = OK b.
+  
+  Definition fsim_13 : Semantics.forward_simulation (Untyped1.semantics a) (Untyped3.semantics b).
+    eapply Semantics.compose_forward_simulation; try eapply UntypedComp2.fsim; try eapply UntypedComp3.fsim.
+    unfold compile_13 in *. simpl in *. reflexivity.
+    unfold compile_13 in *. simpl in *. congruence.
+  Defined.
+
+  Lemma fsim_13_match_val :
+    forall x y,
+      Semantics.fsim_match_val _ _ fsim_13 x y <-> eq x y.
+  Proof.
+    intros. unfold fsim_13.
+    unfold Semantics.compose_forward_simulation.
+    simpl.
+    erewrite UntypedComp2.match_val_eq.
+    erewrite UntypedComp3.match_val_eq. 
+    split; intros.
+    break_exists; break_and; congruence.
+    eexists; split; eauto.
+  Qed.
+
+End FSIM13.
+
+
+Definition compile_14 (cu : Untyped1.prog_type) : res Untyped4.prog_type :=
+  OK cu
+  @@@ compile_13
+  @@ UntypedComp4.compile_cu.
+
+Section FSIM14.
+
+
+  Variable a : Untyped1.prog_type.
+  Variable b : Untyped4.prog_type.
+  Hypothesis TRANSF : compile_14 a = OK b.
+  
+  Definition fsim_14 : Semantics.forward_simulation (Untyped1.semantics a) (Untyped4.semantics b).
+    eapply Semantics.compose_forward_simulation; try eapply fsim_13; try eapply UntypedComp4.fsim.
+    unfold compile_14 in *. simpl in *. reflexivity.
+    unfold compile_14 in *. simpl in *. congruence.
+  Defined.
+
+  Lemma fsim_14_match_val :
+    forall x y,
+      Semantics.fsim_match_val _ _ fsim_14 x y <-> eq x y.
+  Proof.
+    intros. unfold fsim_14.
+    erewrite Semantics.fsim_match_val_compose. repeat instantiate (1 := eq).
+    split; intros; repeat break_exists; repeat eexists; repeat break_and; eauto; try congruence.
+    eapply fsim_13_match_val.
+    erewrite UntypedComp4.match_val_eq. intros.
+    split; intros; congruence.
+  Qed.
+
+End FSIM14.
+
+
+Definition compile_15 (cu : Untyped1.prog_type) : res Untyped5.prog_type :=
+  OK cu
+  @@@ compile_14
+  @@@ UntypedComp5.compile_cu.
+
+Section FSIM15.
+
+
+  Variable a : Untyped1.prog_type.
+  Variable b : Untyped5.prog_type.
+  Hypothesis TRANSF : compile_15 a = OK b.
+  
+  Definition fsim_15 : Semantics.forward_simulation (Untyped1.semantics a) (Untyped5.semantics b).
+    eapply Semantics.compose_forward_simulation; try eapply fsim_14; try eapply UntypedComp5.fsim.
+    unfold compile_15 in *. simpl in *. reflexivity.
+    unfold compile_15 in *. simpl in *. unfold option_to_res in *. break_match_hyp; try congruence.
+    inv TRANSF. reflexivity.
+  Defined.
+
+  Lemma fsim_15_match_val :
+    forall x y,
+      Semantics.fsim_match_val _ _ fsim_15 x y <-> eq x y.
+  Proof.
+    intros. unfold fsim_15.
+    erewrite Semantics.fsim_match_val_compose. repeat instantiate (1 := eq).
+    split; intros; repeat break_exists; repeat eexists; repeat break_and; eauto; try congruence.
+    eapply fsim_14_match_val.
+    erewrite UntypedComp5.match_val_eq. intros.
+    split; intros; congruence.
+  Qed.
+
+End FSIM15.
+
+
+Definition compile_16 (cu : Untyped1.prog_type) : res Untyped6.prog_type :=
+  OK cu
+  @@@ compile_15
+  @@ UntypedComp6.compile_cu.
+
+Section FSIM16.
+
+
+  Variable a : Untyped1.prog_type.
+  Variable b : Untyped6.prog_type.
+  Hypothesis TRANSF : compile_16 a = OK b.
+
+  Lemma compile_16_succ :
+    { c | compile_15 a = OK c }.
+  Proof.
+    unfold compile_16 in TRANSF. break_result_chain. eauto.
+  Qed.
+  
+  Definition fsim_16 : Semantics.forward_simulation (Untyped1.semantics a) (Untyped6.semantics b).
+    destruct compile_16_succ.
+    eapply Semantics.compose_forward_simulation;
+      try eapply fsim_15;
+      try eapply UntypedComp6.fsim; eauto.
+    unfold compile_16 in *; break_result_chain.
+    congruence.
+  Defined.
+
+  Lemma fsim_16_match_val :
+    forall x y,
+      Semantics.fsim_match_val _ _ fsim_16 x y <-> eq x y.
+  Proof.
+    intros. unfold fsim_16.
+    destruct compile_16_succ.
+    erewrite Semantics.fsim_match_val_compose. repeat instantiate (1 := eq).
+    split; intros; repeat break_exists; repeat eexists; repeat break_and; eauto; try congruence.
+    eapply fsim_15_match_val.
+    erewrite UntypedComp6.match_val_eq. intros.
+    split; intros; congruence.
+  Qed.
+
+End FSIM16.
+
+Definition compile_17 (cu : Untyped1.prog_type) : res Untyped7.prog_type :=
+  OK cu
+  @@@ compile_16
+  @@@ UntypedComp7.compile_cu.
+
+Section FSIM17.
+
+
+  Variable a : Untyped1.prog_type.
+  Variable b : Untyped7.prog_type.
+  Hypothesis TRANSF : compile_17 a = OK b.
+
+  Lemma compile_17_succ :
+    { c | compile_16 a = OK c }.
+  Proof.
+    unfold compile_17 in TRANSF. break_result_chain. eauto.
+  Qed.
+  
+  Definition fsim_17 : Semantics.forward_simulation (Untyped1.semantics a) (Untyped7.semantics b).
+    destruct compile_17_succ.
+    eapply Semantics.compose_forward_simulation;
+      try eapply fsim_16;
+      try eapply UntypedComp7.fsim; eauto.
+    unfold compile_17 in *; break_result_chain.
+    congruence.
+  Defined.
+
+  Lemma fsim_17_match_val :
+    forall x y,
+      Semantics.fsim_match_val _ _ fsim_17 x y <-> eq x y.
+  Proof.
+    intros. unfold fsim_17.
+    destruct compile_17_succ.
+    erewrite Semantics.fsim_match_val_compose. repeat instantiate (1 := eq).
+    split; intros; repeat break_exists; repeat eexists; repeat break_and; eauto; try congruence.
+    eapply fsim_16_match_val.
+    erewrite UntypedComp7.match_val_eq. intros.
+    split; intros; congruence.
+  Qed.
+
+End FSIM17.
+
+
+Definition compile_18 (cu : Untyped1.prog_type) : res Untyped8.prog_type :=
+  OK cu
+  @@@ compile_17
+  @@ UntypedComp8.compile_cu.
+
+Section FSIM18.
+
+
+  Variable a : Untyped1.prog_type.
+  Variable b : Untyped8.prog_type.
+  Hypothesis TRANSF : compile_18 a = OK b.
+
+  Lemma compile_18_succ :
+    { c | compile_17 a = OK c }.
+  Proof.
+    unfold compile_18 in TRANSF. break_result_chain. eauto.
+  Qed.
+  
+  Definition fsim_18 : Semantics.forward_simulation (Untyped1.semantics a) (Untyped8.semantics b).
+    destruct compile_18_succ.
+    eapply Semantics.compose_forward_simulation;
+      try eapply fsim_17;
+      try eapply UntypedComp8.fsim; eauto.
+    unfold compile_18 in *; break_result_chain.
+    congruence.
+  Defined.
+
+  Lemma fsim_18_match_val :
+    forall x y,
+      Semantics.fsim_match_val _ _ fsim_18 x y <-> eq x y.
+  Proof.
+    intros. unfold fsim_18.
+    destruct compile_18_succ.
+    erewrite Semantics.fsim_match_val_compose. repeat instantiate (1 := eq).
+    split; intros; repeat break_exists; repeat eexists; repeat break_and; eauto; try congruence.
+    eapply fsim_17_match_val.
+    erewrite UntypedComp8.match_val_eq. intros.
+    split; intros; congruence.
+  Qed.
+
+End FSIM18.
+
+
 Module A := Untyped1.
 Module B := Untyped8.
 
-Definition compile_cu (cu : A.env * list metadata) : res (B.env * list metadata) :=
-  OK cu
-  @@ UntypedComp2.compile_cu
-  @@ UntypedComp3.compile_cu
-  @@ UntypedComp4.compile_cu
- @@@ UntypedComp5.compile_cu
-  @@ UntypedComp6.compile_cu
- @@@ UntypedComp7.compile_cu
-  @@ UntypedComp8.compile_cu
-.
+Definition compile_cu (cu : A.env * list metadata) : res (B.env * list metadata) := compile_18 cu.
 
-
-
-Require Semantics.
 
 Section Preservation.
 
@@ -43,29 +265,19 @@ Variable bprog : B.prog_type.
 
 Hypothesis Hcomp : compile_cu aprog = OK bprog.
 
-Theorem fsim : Semantics.forward_simulation (A.semantics aprog) (B.semantics bprog).
-    unfold compile_cu in Hcomp.
-    break_result_chain.
+Definition fsim : Semantics.forward_simulation (A.semantics aprog) (B.semantics bprog).
+  eapply fsim_18. eapply Hcomp.
+Defined.
 
-    eapply Semantics.compose_forward_simulation.
-    eapply UntypedComp2.fsim; try eassumption.
-
-    eapply Semantics.compose_forward_simulation.
-    eapply UntypedComp3.fsim; try eassumption.
-
-    eapply Semantics.compose_forward_simulation.
-    eapply UntypedComp4.fsim; try eassumption.
-
-    eapply Semantics.compose_forward_simulation.
-    eapply UntypedComp5.fsim; try eassumption.
-
-    eapply Semantics.compose_forward_simulation.
-    eapply UntypedComp6.fsim; try eassumption.
-
-    eapply Semantics.compose_forward_simulation.
-    eapply UntypedComp7.fsim; try eassumption.
-
-    eapply UntypedComp8.fsim; try eassumption.
+Lemma fsim_match_val :
+  forall x y,
+    Semantics.fsim_match_val _ _ fsim x y <-> x = y.
+Proof.
+  intros. unfold fsim. erewrite fsim_18_match_val. split; intros; congruence.
 Qed.
 
+
 End Preservation.
+
+
+  
